Rename definitions to more closely match the paper

LambdaGraph/Basic.lean
@@ -21,19 +21,19 @@ inductive Ty where
 /--
 A collection of labelled lambda terms.
 
-An environment is represented as an array of function bodies and an array of the
+A program is represented as an array of function bodies and an array of the
 types of their corresponding variables.
 -/
-structure Env where
+structure Program where
   size : Nat
   /-- Maps each label to the corresponding function body. -/
   fn : Vector Expr size
   /-- Maps each label to the type of the corresponding function's argument. -/
   ty : Vector Ty size
 
-/-- A program consists of an environment and an expression to be evaluated. -/
+/-- A computation consists of a program and an expression to be evaluated. -/
 @[pp_using_anonymous_constructor]
-structure Program extends Env where
+structure Computation extends Program where
   /-- The expression to be evaluated. -/
   expr : Expr
 
@@ -44,7 +44,7 @@ A variable occurs free in an expression if the expression itself contains the
 variable, or if it contains a reference to a function in which the variable
 occurs free.
 -/
-inductive Expr.Free (p : Env) (n : Nat) : Expr → Prop where
+inductive Expr.Free (p : Program) (n : Nat) : Expr → Prop where
   | var : Free p n (.var n)
   | fn (m : Nat) (_ : m < p.size) : n ≠ m → Free p n p.fn[m] → Free p n (.fn m)
   | appL (f e : Expr) : Free p n f → Free p n (.app f e)
@@ -54,29 +54,29 @@ inductive Expr.Free (p : Env) (n : Nat) : Expr → Prop where
   | condF (c et ef : Expr) : Free p n ef → Free p n (.cond c et ef)
 
 /--
-A dependency of a function on a variable.
+The nesting relation between functions in a program.
 
-During substitution, all functions that depend on the substitution variable must
-be rewritten.
+During substitution, all functions nested in the function corresponding to the
+substitution variable must be rewritten.
 -/
-inductive Depends (p : Env) : Nat → Nat → Prop where
-  | free (m n : Nat) (_ : m < p.size) : n ≠ m → p.fn[m].Free p n → Depends p m n
-  | step (m n k : Nat) (_ : m < p.size) :
-    n ≠ m → p.fn[m].Free p n → Depends p n k → Depends p m k
+inductive Nests (p : Program) (n : Nat) : Nat → Prop where
+  | free (m : Nat) (_ : m < p.size) : n ≠ m → p.fn[m].Free p n → Nests p n m
+  | step (m k : Nat) (_ : k < p.size) :
+    m ≠ k → p.fn[k].Free p m → Nests p n m → Nests p n k
 
 /-- An expression is closed if it has no free variables. -/
-def Expr.Closed (p : Env) (e : Expr) : Prop := ∀ n, ¬e.Free p n
+def Expr.Closed (p : Program) (e : Expr) : Prop := ∀ n, ¬e.Free p n
 
 /--
-Free variables of a program.
+Free variables of a computation.
 
-A variable occurs free in a program if it occurs free in the program's
+A variable occurs free in a computation if it occurs free in the computation's
 expression.
 -/
-def Program.Free (p : Program) (n : Nat) := p.expr.Free p.toEnv n
+def Computation.Free (p : Computation) (n : Nat) := p.expr.Free p.toProgram n
 
-/-- A program is closed if its expression is closed in its environment. -/
-def Program.Closed (p : Program) : Prop := ∀ n, ¬p.Free n
+/-- A computation is closed if its expression is closed in its program. -/
+def Computation.Closed (p : Computation) : Prop := ∀ n, ¬p.Free n
 
 /--
 A mapping from old labels to new labels assigned for substitution.
@@ -84,20 +84,20 @@ A mapping from old labels to new labels assigned for substitution.
 There is also a mapping that maps the newly assigned labels back to their
 original labels.
 -/
-structure LabelMap (p : Env) where
+structure LabelMap (p : Program) where
   fwd : Vector Nat p.size
   inv : Array (Fin p.size)
 
 open Classical in -- TODO: Remove this by implementing Decidable.
 /-- Returns a label map to use for substitution of the variable `n`. -/
-noncomputable def Env.labelMap (p : Env) (n : Nat) :
+noncomputable def Program.labelMap (p : Program) (n : Nat) :
     LabelMap p :=
   let (fwd, inv) := aux 0 (Vector.ofFn Fin.val) #[]
   ⟨fwd, inv⟩
 where
   aux i map inv :=
     if h : i < p.size then
-      if Depends p i n then
+      if Nests p n i then
         aux (i + 1) (map.set i (p.size + inv.size)) (inv.push ⟨i, h⟩)
       else
         aux (i + 1) map inv
@@ -107,13 +107,13 @@ where
 /--
 Substitutes a value for a variable in an expression.
 
-The expression may include references to functions that include the variable to
-be substituted as a free variable. For these functions, new versions need to be
-added to the environment, with their free occurrences substituted as well. This
-function does not perform this change to the environment, but takes a label map
+The expression may include references to functions nested inside the function
+corresponding to the substitution variable. For these functions, new versions
+need to be added to the program, with their bodies substituted in the same way.
+This function does not perform this change to the program, but takes a label map
 mapping function labels to the labels assigned to their substituted versions.
 -/
-noncomputable def Expr.subst {p : Env} (e : Expr) (map : LabelMap p)
+noncomputable def Expr.subst {p : Program} (e : Expr) (map : LabelMap p)
     (n : Nat) (v : Expr) : Expr :=
   match e with
   | var m => if n = m then v else var (map.fwd[m]?.getD m)
@@ -123,13 +123,13 @@ noncomputable def Expr.subst {p : Env} (e : Expr) (map : LabelMap p)
   | cond c et ef => (c.subst map n v).cond (et.subst map n v) (ef.subst map n v)
 
 /--
-Substitutes a value for a variable in an environment.
+Substitutes a value for a variable in a program.
 
 This creates a new version of each function that depends on `n`, as specified by
 the passed label map.
 -/
-noncomputable def Env.subst (p : Env) (map : LabelMap p) (n : Nat) (v : Expr) :
-    Env :=
+noncomputable def Program.subst (p : Program) (map : LabelMap p) (n : Nat) (v : Expr) :
+    Program :=
   let fnExt : Vector Expr map.inv.size :=
     ⟨map.inv.map (p.fn[·].subst map n v), by simp⟩
   let tyExt : Vector Ty map.inv.size :=
@@ -137,14 +137,14 @@ noncomputable def Env.subst (p : Env) (map : LabelMap p) (n : Nat) (v : Expr) :
   { size := _, fn := p.fn ++ fnExt, ty := p.ty ++ tyExt }
 
 /--
-Substitutes a value for a variable in a program.
+Substitutes a value for a variable in a computation.
 
 This computes the map for translating old labels into new ones and applies the
-substitution to the environment and the expression.
+substitution to the program and the expression.
 -/
-noncomputable def Program.subst (p : Program) (n : Nat) (v : Expr) : Program :=
+noncomputable def Computation.subst (p : Computation) (n : Nat) (v : Expr) : Computation :=
   let map := p.labelMap n
-  ⟨p.toEnv.subst map n v, p.expr.subst map n v⟩
+  ⟨p.toProgram.subst map n v, p.expr.subst map n v⟩
 
 /-- A fully reduced expression. -/
 inductive Expr.Value : Expr → Prop where
@@ -152,37 +152,37 @@ inductive Expr.Value : Expr → Prop where
   | bool b : Value (.bool b)
 
 /-- The small-step reduction relation. -/
-inductive Step : Program → Program → Prop where
-  | app (p : Env) (n : Nat) (e : Expr) (_ : n < p.size) :
-    e.Value → Step ⟨p, .app (.fn n) e⟩ (Program.subst ⟨p, p.fn[n]⟩ n e)
-  | appL (p p' : Env) (f f' e : Expr) :
+inductive Step : Computation → Computation → Prop where
+  | app (p : Program) (n : Nat) (e : Expr) (_ : n < p.size) :
+    e.Value → Step ⟨p, .app (.fn n) e⟩ (Computation.subst ⟨p, p.fn[n]⟩ n e)
+  | appL (p p' : Program) (f f' e : Expr) :
     Step ⟨p, f⟩ ⟨p', f'⟩ → Step ⟨p, f.app e⟩ ⟨p', f'.app e⟩
-  | appR (p p' : Env) (f e e' : Expr) :
+  | appR (p p' : Program) (f e e' : Expr) :
     f.Value → Step ⟨p, e⟩ ⟨p', e'⟩ → Step ⟨p, f.app e⟩ ⟨p', f.app e'⟩
-  | condT (p : Env) (et ef : Expr) :
+  | condT (p : Program) (et ef : Expr) :
     Step ⟨p, (.cond (.bool true) et ef)⟩ ⟨p, et⟩
-  | condF (p : Env) (et ef : Expr) :
+  | condF (p : Program) (et ef : Expr) :
     Step ⟨p, (.cond (.bool false) et ef)⟩ ⟨p, ef⟩
-  | condC (p p' : Env) (c c' et ef : Expr) :
+  | condC (p p' : Program) (c c' et ef : Expr) :
     Step ⟨p, c⟩ ⟨p', c'⟩ → Step ⟨p, c.cond et ef⟩ ⟨p', c'.cond et ef⟩
 
 notation:40 p:41 " ⇒ " p':41 => Step p p'
 
 /-- The reflexive-transitive closure of the reduction relation. -/
-inductive Steps : Program → Program → Prop where
-  | refl (p : Program) : Steps p p
-  | step (p p' p'' : Program) : Step p p' → Steps p' p'' → Steps p p''
+inductive Steps : Computation → Computation → Prop where
+  | refl (p : Computation) : Steps p p
+  | step (p p' p'' : Computation) : Step p p' → Steps p' p'' → Steps p p''
 
 notation:40 p:41 " ⇒* " p':41 => Steps p p'
 
 /--
 The typing relation on expressions.
 
-The expression is parameterised by the environment, which contains the typing
+The relation is parameterised by the program, which contains the typing
 information for all variables and functions. Variables and functions are only
 well-typed if their labels are in bounds.
 -/
-inductive Expr.Types (p : Env) : Expr → Ty → Prop where
+inductive Expr.Types (p : Program) : Expr → Ty → Prop where
   | var (n : Nat) (_ : n < p.size) : Types p (var n) p.ty[n]
   | fn (n : Nat) (_ : n < p.size) : Types p (fn n) p.ty[n].cn
   | app (f e : Expr) (t : Ty) :
@@ -194,22 +194,22 @@ inductive Expr.Types (p : Env) : Expr → Ty → Prop where
 notation:60 p:61 " ⊢ " e:61 " : " t:61 => Expr.Types p e t
 
 /--
-The typing predicate for environments.
+The typing predicate for programs.
 
-An environment is well-typed if all function bodies are well-typed.
+A program is well-typed if all function bodies are well-typed.
 -/
-def Env.Types (p : Env) : Prop := ∀ {n}, (_ : n < p.size) → p ⊢ p.fn[n] : .bot
+def Program.Types (p : Program) : Prop := ∀ {n}, (_ : n < p.size) → p ⊢ p.fn[n] : .bot
 
-notation:60 "⊢ " p:61 => Env.Types p
+notation:60 "⊢ " p:61 => Program.Types p
 
 /--
-The typing relation on programs.
+The typing relation on computations.
 
-A program is well-typed if the environment is well-typed and the expression is
-well-typed in that context.
+A computation is well-typed if the program is well-typed and the expression is
+well-typed in that program.
 -/
-structure Program.Types (p : Program) (t : Ty) : Prop where
-  env_types : ⊢ p.toEnv
-  expr_types : p.toEnv ⊢ p.expr : t
+structure Computation.Types (p : Computation) (t : Ty) : Prop where
+  program_types : ⊢ p.toProgram
+  expr_types : p.toProgram ⊢ p.expr : t
 
-notation:60 "⊢ " p:61 " : " t:61 => Program.Types p t
+notation:60 "⊢ " p:61 " : " t:61 => Computation.Types p t
